Added Test data

Source/EdsgerTests/TestData/BresenhamTest.bpl
@@ -1,9 +1,9 @@
-function abs(x: int): int
+function {:inline 5} abs(x: int): int
 {
    if x < 0 then -x else x
 }
  
-//function {:synthesize} f(A: int, B: int, x: int, y: int) returns (int);
+function {:synthesize} f(A: int, B: int, e: int) returns (int);
 
 procedure Bresenham(A: int, B: int)
 requires (0 <= B && B <= A);
@@ -11,25 +11,31 @@ requires (0 <= B && B <= A);
     var x: int; var y: int; var e: int;
     
     e := 2 * B - A;
-    x, y := 0, 0;
+    y := 0;
+    x := 0;
     
     while (x <= A)
     invariant e == 2 * (x + 1) * B - (2 * y + 1) * A;
     invariant 2 * (B - A) <= e && e <= 2 * B;
+    invariant 2 * abs(A * y - B * x) <= A;
     {
         // Mark the point.
-        assert 2 * abs(A * y - B * x) <= A;
+        //assert 2 * abs(A * y - B * x) <= A;
         
         if (e < 0) 
         {
             e := e + 2 * B;
+            assert 2 * abs(A * y - B * (x + 1)) <= A;            
         }
         else
         {
-            e := e + 2 * (B - A);
+            //e := e + 2 * (B - A);
+            e := f(A, B, e);
             y := y + 1;
+            assert 2 * abs(A * y - B * (x + 1)) <= A;            
         }
         x := x + 1;
+        //assert 2 * abs(A * y - B * x) <= A;
     } 
 }
 
