Source/EdsgerTests/TestData/DutchNationalFlag.bpl
@@ -1,10 +1,51 @@
+// ensures ((exists p: int, q: int | 0 <= p && p <= q && q <= N :: (forall i: int | 0 <= i && i < p :: arr[i] == 0) && 
+//                                                                 (forall i: int | p <= i && i < q :: arr[i] == 1) &&
+//                                                                 (forall i: int | q <= i && i < N :: arr[i] == 2) );
 
-procedure DutchNationalFlag(arr: [int]int, N: int) returns (r: int)
+
+var arr: [int]int;
+var N: int;
+
+procedure Swap(x: int, y: int)
+modifies arr;
+ensures arr[x] == old(arr)[y];
+ensures arr[y] == old(arr)[x];
+ensures (forall i: int :: i != x && i != y ==> arr[i] == old(arr)[i]);
+{
+    var tmp: int;
+    tmp := arr[x];
+    arr[x] := arr[y];
+    arr[y] := tmp;
+}
+
+procedure DutchNationalFlag() returns (r: int, w: int)
+modifies arr;
 requires (0 <= N);
-ensures ((exists p: int, q: int | 0 <= p <= q <= N :: (forall i: int | 0 <= i < p :: arr[i] == 0) && 
-                                                      (forall i: int | p <= i < q :: arr[i] == 1) &&
-                                                      (forall i: int | q <= i < N :: arr[i] == 2) );
+requires (forall i: int :: 0 <= i && i < N ==> arr[i] == 1 || arr[i] == 2 || arr[i] == 3);
+ensures 0 <= r && r <= w && w <= N;
+ensures (forall i: int :: 0 <= i && i < r ==> arr[i] == 1);
+ensures (forall i: int :: r <= i && i < w ==> arr[i] == 2);
+ensures (forall i: int :: w <= i && i < N ==> arr[i] == 3);
 {    
-
+    var b: int;
+    r, w, b := 0, 0, N;
+    
+    while (w != b)
+    invariant (forall i: int :: 0 <= i && i < r ==> arr[i] == 1);
+    invariant (forall i: int :: r <= i && i < w ==> arr[i] == 2);
+    invariant (forall i: int :: b <= i && i < N ==> arr[i] == 3);
+    invariant 0 <= r && r <= w && w <= b && b <= N;
+    {
+        if (arr[w] == 1) {
+            call Swap(w, r);
+            r := r + 1;
+            w := w + 1;
+        } else if (arr[w] == 2){
+            w := w + 1;
+        } else if (arr[w] == 3){
+            call Swap(w, b-1);
+            b := b -1;
+        }
+    }
   
 }
