Source/EdsgerTests/Edsger/DivMod_01.bpl
@@ -1,10 +1,9 @@
 
 procedure DivMod(a: int, b: int) returns (q: int, r: int);
-requires (a >= 0 && b > 0);
-ensures (a == q * b + r && 0 <= r && r < b);
-
+requires a >= 0 && b > 0;
+ensures a == q * b + r && 0 <= r && r < b;
 
 implementation DivMod(a: int, b: int) returns (q: int, r: int)
 {
-    assume(a == q * b + r && 0 <= r && r < b);    
+    assume a == q * b + r && 0 <= r && r < b;
 }
