Source/EdsgerTests/Edsger/DivMod_02.bpl
@@ -1,15 +1,15 @@
 
 procedure DivMod(a: int, b: int) returns (q: int, r: int);
-requires (a >= 0 && b > 0);
-ensures (a == q * b + r && 0 <= r && r < b);
-{    
+requires a >= 0 && b > 0;
+ensures a == q * b + r && 0 <= r && r < b;
 
-  assume(a == q * b + r && 0 <= r);    
-  
-  while (r >= b)
-  invariant (a == q * b + r && 0 <= r);  
-  {
-    
-  }
-  
+implementation DivMod(a: int, b: int) returns (q: int, r: int)
+{    
+    assume a == q * b + r && 0 <= r;
+    while (r >= b)
+    invariant a == q * b + r && 0 <= r;
+    {
+        // Loop Body
+        assume a == q * b + r && 0 <= r;
+    }
 }
