Source/EdsgerTests/Edsger/DivMod_03.bpl
@@ -1,19 +1,21 @@
+function {:synthesize} f(r: int, a: int, b: int) returns (int) {r - b}
 
+procedure DivMod(a: int, b: int) returns (q: int, r: int);
+requires a >= 0 && b > 0;
+ensures a == q * b + r && 0 <= r && r < b;
 
-procedure DivMod(a: int, b: int) returns (q: int, r: int)
-requires (a >= 0 && b > 0);
-ensures (a == q * b + r && 0 <= r && r < b);
-{    
-
-  r := a;
-  q := 0;
-  
-  assert(a == q * b + r && 0 <= r);    
-  
-  while (r >= b)
-  invariant (a == q * b + r && 0 <= r);  
-  {
+implementation DivMod(a: int, b: int) returns (q: int, r: int)
+{   
+    q := 0;
+    r := a;
     
-  }
-  
+    assert a == q * b + r && 0 <= r;
+    
+    while (r >= b)
+    invariant a == q * b + r && 0 <= r;
+    {
+        q := q + 1;
+        r := f(r, a, b);
+        assert a == q * b + r && 0 <= r;
+    }
 }
