Source/EdsgerTests/TestData/BresenhamTest2.bpl
@@ -1,0 +1,36 @@
+function {:inline 5} abs(x: int): int
+{
+   if x < 0 then -x else x
+}
+ 
+function {:synthesize} f(B: int, e: int) returns (int);
+
+procedure Bresenham(A: int, B: int)
+requires (0 <= B && B <= A);
+{
+    var x: int; var y: int; var e: int;
+    
+    e := 2 * B - A;
+    y := 0;
+    x := 0;
+    
+    while (x <= A)
+    invariant e == 2 * (x + 1) * B - (2 * y + 1) * A;
+    invariant 2 * (B - A) <= e && e <= 2 * B;
+    invariant 2 * abs(A * y - B * x) <= A;
+    {
+        // Mark the point.
+        //assert 2 * abs(A * y - B * x) <= A;
+        
+        assume e < 0; 
+        
+        //e := e + 2 * B;
+        e := f(B, e);
+        assert 2 * abs(A * y - B * (x + 1)) <= A;            
+        
+        x := x + 1;
+        //assert 2 * abs(A * y - B * x) <= A;
+    } 
+}
+
+// /Users/dipakc/progs/cvc4_1_8/cvc4_wrapper.sh --lang=sygus2 --no-strict-parsing --no-condense-function-values --produce-models /Users/dipakc/SourceRepos/Edsger/Source/EdsgerTests/TestOutput/_BresenhamCopy.sygus
