Source/EdsgerTests/TestData/BresenhamTest3.bpl
@@ -1,0 +1,38 @@
+function {:inline 5} abs(x: int): int
+{
+   if x < 0 then -x else x
+}
+
+function {:synthesize} f(A: int, B: int, e: int) returns (int);
+
+procedure Bresenham(A: int, B: int)
+requires (0 <= B && B <= A);
+{
+    var x: int; var y: int; var e: int;
+    
+    e := 2 * B - A;
+    y := 0;
+    x := 0;
+    
+    while (x <= A)
+    invariant e == 2 * (x + 1) * B - (2 * y + 1) * A;
+    //invariant 2 * (B - A) <= e && e <= 2 * B;
+    //invariant -A <= 2 * (A * y - B * x) && 2 * (A * y - B * x) <= A;
+    invariant 2 * abs(A * y - B * x) <= A;
+    {
+        // Mark the point.
+        //assert 2 * abs(A * y - B * x) <= A;
+        
+        assume e < 0; 
+        //e := e + 2 * B;
+        e := f(A, B, e);                  
+        
+        //e := e + 2 * (B - A);
+        //y := y + 1;     
+        //assert 2 * abs(A * y - B * (x + 1)) <= A;
+        //assert e == 2 * (x + 2) * B - (2 * y + 1) * A;
+        x := x + 1;
+        //assert 2 * abs(A * y - B * x) <= A;
+    } 
+}
+
