Source/EdsgerTests/TestData/DutchNationalFlag_02.bpl
@@ -1,0 +1,36 @@
+var arr: [int]int;
+var N: int;
+
+procedure Swap(x: int, y: int)
+modifies arr;
+ensures arr[x] == old(arr)[y];
+ensures arr[y] == old(arr)[x];
+ensures (forall i: int :: i != x && i != y ==> arr[i] == old(arr)[i]);
+{
+    var tmp: int;
+    tmp := arr[x];
+    arr[x] := arr[y];
+    arr[y] := tmp;
+}
+
+function color(arr: [int]int, p: int, q: int, c: int) returns (bool)  {
+    (forall i: int :: p <= i && i < q ==> arr[i] == c)
+}
+
+procedure DutchNationalFlag() returns (r: int, w: int)
+modifies arr;
+requires (0 <= N);
+requires (forall i: int :: 0 <= i && i < N ==> arr[i] == 1 || arr[i] == 2 || arr[i] == 3);
+ensures 0 <= r && r <= w && w <= N;
+ensures color(arr, 0, r, 1);
+ensures color(arr, r, w, 2);
+ensures color(arr, w, N, 3);
+{    
+    var b: int;
+
+    assume 0 <= r && r <= w && w <= b && b <= N;
+    assume color(arr, 0, r, 1);
+    assume color(arr, r, w, 2);
+    assume color(arr, b, N, 3);
+    assume b == w;
+}
