Source/EdsgerTests/TestData/SimpleArray.bpl
@@ -1,0 +1,9 @@
+
+var arr: [int]int;
+
+procedure SimpleArray()
+modifies arr;
+ensures (arr[0] == 2);
+{    
+    arr[0] := 2;  
+}
