Source/EdsgerTests/TestData/Swap.bpl
@@ -1,0 +1,13 @@
+var arr: [int]int;
+
+procedure Swap(x: int, y: int)
+modifies arr;
+ensures arr[x] == old(arr)[y];
+ensures arr[y] == old(arr)[x];
+ensures (forall i: int :: i != x && i != y ==> arr[i] == old(arr)[i]);
+{
+    var tmp: int;
+    tmp := arr[x];
+    arr[x] := arr[y];
+    arr[y] := tmp;
+}
